Hashmap/List/Defs.lean
@@ -13,10 +13,14 @@ namespace List
 
 def keys : List (Σ a, β a) → List α
   | nil => []
-  | ⟨k, _⟩ :: l => k :: (keys l)
+  | ⟨k, _⟩ :: l => k :: l.keys
 
 /-- The well-formedness predicate for `AssocList` says that keys are pairwise distinct. -/
 structure DistinctKeys [BEq α] (l : List (Σ a, β a)) : Prop where
   distinct : l.keys.Pairwise fun a b => (a == b) = false
+
+def values {β : Type v} : List ((_ : α) × β) → List β
+  | nil => []
+  | ⟨_, v⟩ :: l => v :: l.values
 
 end List
